
## Strong Induction

Weak induction works as the following: $BS + IS(f(m) \implies f(m+1))$
As opposed to strong induction. $BS + IS (\forall k \leq m, f(k) \implies f(m+1))$  
When it is not enough to go one step back, rather we need to go a finite amount of steps back, we have to use a stronger hypothesis - the strong induction. An example for a need of this is when an element is defined recursively by its previous elements.
Note that the BS in strong induction is not for a singular case, but for several.
